src/Lean/Parser/Term.lean
@@ -92,7 +92,8 @@ def bracketedBinder (requireType := false) := explicitBinder requireType <|> imp
 def simpleBinder := parser! many1 binderIdent
 @[builtinTermParser] def «forall» := parser!:leadPrec unicodeSymbol "∀ " "forall " >> many1 (simpleBinder <|> bracketedBinder) >> ", " >> termParser
 
-def funBinder : Parser := implicitBinder <|> instBinder <|> termParser maxPrec
+def funImplicitBinder := try (lookahead ("{" >> many1 binderIdent >> " : ")) >> implicitBinder
+def funBinder : Parser := funImplicitBinder <|> instBinder <|> termParser maxPrec
 @[builtinTermParser] def «fun» := parser!:maxPrec unicodeSymbol "λ " "fun " >> many1 funBinder >> darrow >> termParser
 
 def matchAlt : Parser :=
